Proposition 4.2. 
For statements $p, q, r$, 
(1) p ∧ q ⇔ q ∧ p 
(2) p ∨ q ⇔ q ∨ p 
(3) p ∧ (q ∧ r) ⇔ (p ∧ q) ∧ r 
(4) p ∨ (q ∨ r) ⇔ (p ∨ q) ∨ r 
(5) p ∧ (q ∨ r) ⇔ (p ∧ q) ∨ (p ∧ r) 
(6) p ∨ (q ∧ r) ⇔ (p ∨ q) ∧ (p ∨ r) 
(7) p ∧ p ⇔ p 
(8) p ∨ p ⇔ p 
(9) ¬(¬p) ⇔ p 
(10) ¬(p ∧ q) ⇔ ¬p ∨ ¬q 
(11) ¬(p ∨ q) ⇔ ¬p ∧ ¬q

Proposition 4.3. 
For arbitrary sets $A, B, C$ of a universal set $U$, 
(1) A ∩ B = B ∩ A 
(2) A ∪ B = B ∪ A 
(3) A ∩ (B ∩ C) = (A ∩ B) ∩ C 
(4) A ∪ (B ∪ C) = (A ∪ B) ∪ C 
(5) A ∩ (B ∪ C) = (A ∩ B) ∪ (A ∩ C) 
(6) A ∪ (B ∩ C) = (A ∪ B) ∩ (A ∪ C)
(7) A ∩ A = A 
(8) A ∪ A = A 
![[chrome_6NUKDHbgG3.png]]
*(Line on top of set = complement of the set)*

